messageInvariantPrototypes/clientServer/types.dfy
@@ -16,4 +16,14 @@ module Types {
   }
 
   datatype MessageOps = MessageOps(recv:Option<Message>, send:Option<Message>)
+
+  datatype Transmit = Transmit(m: Message) {
+    function Send() : MessageOps {
+      MessageOps(None, Some(m))
+    }
+
+    function Recv() : MessageOps {
+      MessageOps(Some(m), None)
+    }
+  }
 } // end module Types
