messageInvariantPrototypes/clientServer/centralizedMonotonic_globalHistory/system.dfy
@@ -1,4 +1,4 @@
-include "../centralizedHosts.dfy"
+include "centralizedHosts.dfy"
 
 module System {
 import opened UtilitiesLibrary
